ClassicalLogicLean/NV/Sub/Var/All/Ind/Sub.lean
@@ -256,7 +256,7 @@ theorem substitution_theorem_is_sub_var_all_ind_aux
             exact ih_1 x a2 c3
 
         simp only [s1]
-        apply Function.updateListITE_mem_eq_len
+        apply Function.updateFromPairOfListsITE_mem_eq_len
         simp only [var_is_free_in_iff_mem_free_var_set] at a1
         obtain s2 := hd.h1 a1
         simp at s2
