ClassicalLogicLean/NV/Sub/Var/One/Rec/Admits.lean
@@ -1107,7 +1107,7 @@ theorem substitution_theorem_fast_admits_var_one_rec_aux
           rfl
 
       simp only [s1]
-      apply Function.updateListITE_mem_eq_len
+      apply Function.updateFromPairOfListsITE_mem_eq_len
       · simp only [var_is_free_in_iff_mem_free_var_set] at a1
         simp only [← List.mem_toFinset]
         exact Finset.mem_of_subset hd.h1 a1
