ClassicalLogicLean/NV/Sub/Var/One/Rec/ReplaceFree.lean
@@ -134,7 +134,7 @@ theorem replace_free_var_one_rec_aux_mem_binders
     simp only [replace_free_var_one_rec_aux]
   case pred_const_ X xs | pred_var_ X xs | def_ X xs =>
     simp
-    simp only [List.map_eq_self_iff]
+    simp only [List.map_eq_self_iff_fun_is_id_on_mem]
     simp
     intro x _ a2 a3
     subst a2
@@ -240,7 +240,7 @@ theorem fast_replace_free_var_one_rec_self
     simp only [fast_replace_free_var_one_rec]
   case pred_const_ X xs | pred_var_ X xs | def_ X xs =>
     simp
-    simp only [List.map_eq_self_iff]
+    simp only [List.map_eq_self_iff_fun_is_id_on_mem]
     simp
   case eq_ x y =>
     simp
@@ -271,7 +271,7 @@ theorem not_var_is_free_in_fast_replace_free_var_one_rec_self
     simp only [fast_replace_free_var_one_rec]
   case pred_const_ X xs | pred_var_ X xs | def_ X xs =>
     simp
-    simp only [List.map_eq_self_iff]
+    simp only [List.map_eq_self_iff_fun_is_id_on_mem]
     simp
     intro x a1 a2
     subst a2
@@ -307,7 +307,7 @@ theorem fast_replace_free_var_one_rec_inverse
   case pred_const_ X xs | pred_var_ X xs | def_ X xs =>
     congr!
     simp
-    simp only [List.map_eq_self_iff]
+    simp only [List.map_eq_self_iff_fun_is_id_on_mem]
     simp
     intro x a1
     by_cases c1 : v = x
